Rename box_inv into box_slice_inv.

program_logic/boxes.v
@@ -19,22 +19,22 @@ Section box_defs.
   Definition box_own_prop (γ : gname) (P : iProp) : iProp :=
     own γ (∅:auth _, Some (to_agree (Next (iProp_unfold P)))).
 
-  Definition box_inv (γ : gname) (P : iProp) : iProp :=
+  Definition box_slice_inv (γ : gname) (P : iProp) : iProp :=
     (∃ b, box_own_auth γ (● Excl' b) ★ box_own_prop γ P ★ if b then P else True)%I.
 
   Definition box_slice (γ : gname) (P : iProp) : iProp :=
-    inv N (box_inv γ P).
+    inv N (box_slice_inv γ P).
 
   Definition box (f : gmap gname bool) (P : iProp) : iProp :=
     (∃ Φ : gname → iProp,
       ▷ (P ≡ [★ map] γ ↦ b ∈ f, Φ γ) ★
       [★ map] γ ↦ b ∈ f, box_own_auth γ (◯ Excl' b) ★ box_own_prop γ (Φ γ) ★
-                         inv N (box_inv γ (Φ γ)))%I.
+                         inv N (box_slice_inv γ (Φ γ)))%I.
 End box_defs.
 
 Instance: Params (@box_own_auth) 4.
 Instance: Params (@box_own_prop) 4.
-Instance: Params (@box_inv) 4.
+Instance: Params (@box_slice_inv) 4.
 Instance: Params (@box_slice) 5.
 Instance: Params (@box) 5.
 
@@ -46,7 +46,7 @@ Implicit Types P Q : iProp.
 (* FIXME: solve_proper picks the eq ==> instance for Next. *)
 Global Instance box_own_prop_ne n γ : Proper (dist n ==> dist n) (box_own_prop γ).
 Proof. solve_proper. Qed.
-Global Instance box_inv_ne n γ : Proper (dist n ==> dist n) (box_inv γ).
+Global Instance box_inv_ne n γ : Proper (dist n ==> dist n) (box_slice_inv γ).
 Proof. solve_proper. Qed.
 Global Instance box_slice_ne n γ : Proper (dist n ==> dist n) (box_slice N γ).
 Proof. solve_proper. Qed.
@@ -103,7 +103,7 @@ Proof.
     as {γ} "[Hdom Hγ]"; first done.
   rewrite pair_split. iDestruct "Hγ" as "[[Hγ Hγ'] #HγQ]".
   iDestruct "Hdom" as % ?%not_elem_of_dom.
-  iPvs (inv_alloc N _ (box_inv γ Q) with "[Hγ]") as "#Hinv"; first done.
+  iPvs (inv_alloc N _ (box_slice_inv γ Q) with "[Hγ]") as "#Hinv"; first done.
   { iNext. iExists false. by repeat iSplit. }
   iPvsIntro; iExists γ; repeat iSplit; auto.
   iNext. iExists (<[γ:=Q]> Φ); iSplit.
